Start off the comparisons

Poly1305.Equivalence.fst
@@ -2,3 +2,28 @@ module Poly1305.Equivalence
 
 module ValeSpec = Poly1305.Spec_s
 module HaclSpec = Spec.Poly1305
+
+type nat128 = ValeSpec.nat128
+type size_t = Spec.Lib.IntTypes.size_t   // from HaclSpec
+type lbytes l = Spec.Lib.IntSeq.lbytes l // from HaclSpec
+type key = HaclSpec.key
+type tag = HaclSpec.tag
+
+val spec_equal :
+  key_r:nat128 ->
+  key_s:nat128 ->
+  inp:(int->nat128) ->
+  len:nat ->
+  t:int ->
+  len1:size_t ->
+  msg:lbytes len1 ->
+  k:key ->
+  t1:tag ->
+  Lemma
+    (requires
+       True (* TODO: rewrite this part to make the inputs match up *)
+    )
+    (ensures
+       (ValeSpec.poly1305_hash key_r key_s inp len == t) /\
+     (HaclSpec.poly1305 len1 msg k == t1)
+    )
